Add docstrings to DHashMap/Basic

src/Std/Data/DHashMap/Basic.lean
@@ -11,15 +11,17 @@ import Std.Data.DHashMap.Internal.Defs
 /-!
 # Dependent hash maps
 
-This file develops the two types `Std.Data.DHashMap.Raw` and `Std.Data.DHashMap`. The difference between these
-types is that the former does not bundle the well-formedness invariant and is thus safe to use in
-nested inductive types. The well-formedness predicate is available as `Std.Data.DHashMap.Raw.WF` and this
-file proves that all operations preserve well-formedness.
+This file develops the two types `Std.Data.DHashMap.Raw` and `Std.Data.DHashMap` of dependent hash
+maps. The difference between these types is that the former does not bundle the well-formedness
+invariant and is thus safe to use in nested inductive types. The well-formedness predicate is
+available as `Std.Data.DHashMap.Raw.WF` and this file proves that all operations preserve
+well-formedness. When in doubt, prefer `DHashMap` over `DHashMap.Raw`.
 
-The operations `map` and `filterMap` on `Std.Data.DHashMap` are defined in the module `Std.Data.DHashMap.AdditionalOperations`.
+The operations `map` and `filterMap` on `Std.Data.DHashMap` are defined in the module
+`Std.Data.DHashMap.AdditionalOperations`.
 
-Lemmas about the operations on `Std.Data.DHashMap.Raw` and `Std.Data.DHashMap` are available in the module
-`Std.Data.DHashMap.Lemmas`.
+Lemmas about the operations on `Std.Data.DHashMap` and `Std.Data.DHashMap.Raw` are available in the
+modules `Std.Data.DHashMap.Lemmas` and `Std.Data.DHashMap.RawLemmas`.
 
 For implementation notes, see the docstring of the module `Std.Data.DHashMap.Internal.Defs`.
 -/
@@ -39,39 +41,57 @@ namespace DHashMap
 
 namespace Raw
 
+/-- Creates a new empty hash map. The optional parameter `capacity` can be supplied to presize the
+map so that it can hold the given number of mappings without reallocating. It is also possible to
+use the empty collection notations `∅` and `{}` to create an empty hash map with the default
+capacity. -/
 @[inline] def empty (capacity := 8) : Raw α β :=
   (Raw₀.empty capacity).1
 
 instance : EmptyCollection (Raw α β) where
   emptyCollection := empty
 
+/-- Insert the given mapping into the map, replacing an existing mapping for the key if there is
+one. -/
 @[inline] def insert [BEq α] [Hashable α] (m : Raw α β) (a : α) (b : β a) : Raw α β :=
   if h : 0 < m.buckets.size then
     (Raw₀.insert ⟨m, h⟩ a b).1
   else m -- will never happen for well-formed inputs
 
+/-- If there is no mapping for the given key, insert the given mapping into the map. Otherwise,
+return the map unaltered. -/
 @[inline] def insertIfNew [BEq α] [Hashable α] (m : Raw α β) (a : α) (b : β a) : Raw α β :=
   if h : 0 < m.buckets.size then
     (Raw₀.insertIfNew ⟨m, h⟩ a b).1
   else m -- will never happen for well-formed inputs
 
+/-- Equivalent to (but potentially faster than) calling `contains` followed by `insert`. -/
 @[inline] def containsThenInsert [BEq α] [Hashable α] (m : Raw α β) (a : α) (b : β a) : Bool × Raw α β:=
   if h : 0 < m.buckets.size then
     let ⟨replaced, ⟨r, _⟩⟩ := Raw₀.containsThenInsert ⟨m, h⟩ a b
     ⟨replaced, r⟩
   else (false, m) -- will never happen for well-formed inputs
 
+/-- Equivalent to (but potentially faster than) calling `get?` followed by `insertIfNew`. -/
 @[inline] def getThenInsertIfNew? [BEq α] [Hashable α] [LawfulBEq α] (m : Raw α β) (a : α) (b : β a) : Option (β a) × Raw α β :=
   if h : 0 < m.buckets.size then
     let ⟨previous, ⟨r, _⟩⟩ := Raw₀.getThenInsertIfNew? ⟨m, h⟩ a b
     ⟨previous, r⟩
   else (none, m) -- will never happen for well-formed inputs
 
+/-- Tries to retrieve the mapping for the given key, returning `none` if no such mapping is present.
+
+Uses the `LawfulBEq` instance to cast the retrieved value to the correct type. -/
 @[inline] def get? [BEq α] [LawfulBEq α] [Hashable α] (m : Raw α β) (a : α) : Option (β a) :=
   if h : 0 < m.buckets.size then
     Raw₀.get? ⟨m, h⟩ a
   else none -- will never happen for well-formed inputs
 
+/-- Returns `true` if there is a mapping for the given key. There is also a `Prop`-valued version
+of this: `a ∈ m` is equivalent to `m.contains a = true`.
+
+Observe that this is different behavior than for lists: for lists, `∈` uses `=` and `contains` use
+`==` for comparisons, while for hash maps, both use `==`. -/
 @[inline] def contains [BEq α] [Hashable α] (m : Raw α β) (a : α) : Bool :=
   if h : 0 < m.buckets.size then
     Raw₀.contains ⟨m, h⟩ a
@@ -81,22 +101,36 @@ instance [BEq α] [Hashable α] : Membership α (Raw α β) where
   mem a m := m.contains a
 
 instance [BEq α] [Hashable α] {m : Raw α β} {a : α} : Decidable (a ∈ m) :=
-  show Decidable (m.contains a) from inferInstance
+  inferInstanceAs (Decidable (m.contains a))
 
+/-- Retrieves the mapping for the given key. Ensures that such a mapping exists by requiring a proof
+of `a ∈ m`.
+
+Uses the `LawfulBEq` instance to cast the retrieved value to the correct type. -/
 @[inline] def get [BEq α] [Hashable α] [LawfulBEq α] (m : Raw α β) (a : α) (h : a ∈ m) : β a :=
   Raw₀.get ⟨m, by change dite .. = true at h; split at h <;> simp_all⟩ a
     (by change dite .. = true at h; split at h <;> simp_all)
 
+/-- Tries to retrieve the mapping for the given key, returning `fallback` if no such mapping is
+present.
+
+Uses the `LawfulBEq` instance to cast the retrieved value to the correct type. -/
 @[inline] def getD [BEq α] [Hashable α] [LawfulBEq α] (m : Raw α β) (a : α) (fallback : β a) : β a :=
   if h : 0 < m.buckets.size then
     Raw₀.getD ⟨m, h⟩ a fallback
   else fallback -- will never happen for well-formed inputs
 
+/-- Tries to retrieve the mapping for the given key, panicking if no such mapping is present.
+
+Uses the `LawfulBEq` instance to cast the retrieved value to the correct type. -/
 @[inline] def get! [BEq α] [Hashable α] [LawfulBEq α] (m : Raw α β) (a : α) [Inhabited (β a)] : β a :=
   if h : 0 < m.buckets.size then
     Raw₀.get! ⟨m, h⟩ a
   else default -- will never happen for well-formed inputs
 
+/-- Removes the mapping for the given key if it exists.
+
+Uses the `LawfulBEq` instance to cast the retrieved value to the correct type. -/
 @[inline] def remove [BEq α] [Hashable α] (m : Raw α β) (a : α) : Raw α β :=
   if h : 0 < m.buckets.size then
     Raw₀.remove ⟨m, h⟩ a
@@ -106,25 +140,33 @@ section
 
 variable {β : Type v}
 
+/-- Tries to retrieve the mapping for the given key, returning `none` if no such mapping is present.
+-/
 @[inline] def Const.get? [BEq α] [Hashable α] (m : Raw α (fun _ => β)) (a : α) : Option β :=
   if h : 0 < m.buckets.size then
     Raw₀.Const.get? ⟨m, h⟩ a
   else none -- will never happen for well-formed inputs
 
+/-- Retrieves the mapping for the given key. Ensures that such a mapping exists by requiring a proof
+of `a ∈ m`. -/
 @[inline] def Const.get [BEq α] [Hashable α] (m : Raw α (fun _ => β)) (a : α) (h : a ∈ m) : β :=
   Raw₀.Const.get ⟨m, by change dite .. = true at h; split at h <;> simp_all⟩ a
     (by change dite .. = true at h; split at h <;> simp_all)
 
+/-- Tries to retrieve the mapping for the given key, returning `fallback` if no such mapping is
+present. -/
 @[inline] def Const.getD [BEq α] [Hashable α] (m : Raw α (fun _ => β)) (a : α) (fallback : β) : β :=
   if h : 0 < m.buckets.size then
     Raw₀.Const.getD ⟨m, h⟩ a fallback
   else fallback -- will never happen for well-formed inputs
 
+/-- Tries to retrieve the mapping for the given key, panicking if no such mapping is present. -/
 @[inline] def Const.get! [BEq α] [Hashable α] [Inhabited β] (m : Raw α (fun _ => β)) (a : α) : β :=
   if h : 0 < m.buckets.size then
     Raw₀.Const.get! ⟨m, h⟩ a
   else default -- will never happen for well-formed inputs
 
+/-- Equivalent to (but potentially faster than) calling `Const.get?` followed by `insertIfNew`. -/
 @[inline] def Const.getThenInsertIfNew? [BEq α] [Hashable α] (m : Raw α (fun _ => β)) (a : α) (b : β) :
     Option β × Raw α (fun _ => β) :=
   if h : 0 < m.buckets.size then
@@ -134,6 +176,11 @@ variable {β : Type v}
 
 end
 
+/-- Returns `true` if the hash map contains no mappings.
+
+Note that if your `BEq` instance is not reflexive or your `Hashable` instance is not
+lawful, then it is possible that this function returns `false` even though is not possible
+to get anything out of the hash map. -/
 @[inline] def isEmpty (m : Raw α β) : Bool :=
   m.size == 0
 
@@ -141,16 +188,20 @@ section Unverified
 
 /-! We currently do not provide lemmas for the functions below. -/
 
+/-- Updates the values of the hash map by applying the given function to all mappings, keeping
+only those mappings where the function returns `some` value. -/
 @[inline] def filterMap {γ : α → Type w} (f : (a : α) → β a → Option (γ a)) (m : Raw α β) : Raw α γ :=
   if h : 0 < m.buckets.size then
     Raw₀.filterMap f ⟨m, h⟩
   else ∅ -- will never happen for well-formed inputs
 
+/-- Updates the values of the hash map by applying the given function to all mappings. -/
 @[inline] def map {γ : α → Type w} (f : (a : α) → β a → γ a) (m : Raw α β) : Raw α γ :=
   if h : 0 < m.buckets.size then
     Raw₀.map f ⟨m, h⟩
   else ∅ -- will never happen for well-formed inputs
 
+/-- Removes all mappings of the hash map for which the given function returns `false`. -/
 @[inline] def filter (f : (a : α) → β a → Bool) (m : Raw α β) : Raw α β :=
   if h : 0 < m.buckets.size then
     Raw₀.filter f ⟨m, h⟩
@@ -164,9 +215,11 @@ section Unverified
 @[inline] def foldl (f : δ → (a : α) → β a → δ) (init : δ) (b : Raw α β) : δ :=
   Id.run (b.foldlM f init)
 
+/-- Folds the given function over the mappings in the hash map in some order. -/
 @[inline] def forM (f : (a : α) → β a → m PUnit) (b : Raw α β) : m PUnit :=
   b.buckets.forM (AssocList.forM f)
 
+/-- Support for the `for` loop construct in `do` blocks. -/
 @[inline] def forIn (f : (a : α) → β a → δ → m (ForInStep δ)) (init : δ) (b : Raw α β) : m δ :=
   b.buckets.forIn init (fun bucket acc => bucket.forInStep acc f)
 
@@ -176,51 +229,62 @@ instance : ForM m (Raw α β) (Σ a, β a) where
 instance : ForIn m (Raw α β) (Σ a, β a) where
   forIn m init f := m.forIn (fun a b acc => f ⟨a, b⟩ acc) init
 
+/-- Transforms the hash map into a list of mappings in some order. -/
 @[inline] def toList (m : Raw α β) : List (Σ a, β a) :=
   m.foldl (fun acc k v => ⟨k, v⟩ :: acc) []
 
+/-- Transforms the hash map into an array of mappings in some order. -/
 @[inline] def toArray (m : Raw α β) : Array (Σ a, β a) :=
   m.foldl (fun acc k v => acc.push ⟨k, v⟩) #[]
 
-@[inline] def Const.toList {β : Type v} (m : Raw α (fun _ => β)) : List (α × β) :=
+@[inline, inherit_doc Raw.toList] def Const.toList {β : Type v} (m : Raw α (fun _ => β)) : List (α × β) :=
   m.foldl (fun acc k v => ⟨k, v⟩ :: acc) []
 
-@[inline] def Const.toArray {β : Type v} (m : Raw α (fun _ => β)) : Array (α × β) :=
+@[inline, inherit_doc Raw.toArray] def Const.toArray {β : Type v} (m : Raw α (fun _ => β)) : Array (α × β) :=
   m.foldl (fun acc k v => acc.push ⟨k, v⟩) #[]
 
+/-- Returns a list of all keys present in the hash map in some order. -/
 @[inline] def keys (m : Raw α β) : List α :=
   m.foldl (fun acc k _ => k :: acc) []
 
+/-- Returns an array of all keys present in the hash map in some order. -/
 @[inline] def keysArray (m : Raw α β) : Array α :=
   m.foldl (fun acc k _ => acc.push k) #[]
 
+/-- Returns a list of all values present in the hash map in some order. -/
 @[inline] def values {β : Type v} (m : Raw α (fun _ => β)) : List β :=
   m.foldl (fun acc _ v => v :: acc) []
 
+/-- Inserts multiple mappings into the hash map by iterating over the given collection and calling
+`insert`. If the same key appears multiple times, the last occurrence takes precendence. -/
 @[inline] def insertMany [BEq α] [Hashable α] {ρ : Type w} [ForIn Id ρ ((a : α) × β a)] (m : Raw α β) (l : ρ) : Raw α β :=
   if h : 0 < m.buckets.size then
     (Raw₀.insertMany ⟨m, h⟩ l).1
-else m -- will never happen for well-formed inputs
+  else m -- will never happen for well-formed inputs
 
-@[inline] def Const.insertMany {β : Type v} [BEq α] [Hashable α] {ρ : Type w} [ForIn Id ρ (α × β)] (m : Raw α (fun _ => β)) (l : ρ) : Raw α (fun _ => β) :=
+@[inline, inherit_doc Raw.insertMany] def Const.insertMany {β : Type v} [BEq α] [Hashable α] {ρ : Type w} [ForIn Id ρ (α × β)] (m : Raw α (fun _ => β)) (l : ρ) : Raw α (fun _ => β) :=
   if h : 0 < m.buckets.size then
     (Raw₀.Const.insertMany ⟨m, h⟩ l).1
   else m -- will never happen for well-formed inputs
 
-@[inline] def Const.insertManyUnit [BEq α] [Hashable α] {ρ : Type w} [ForIn Id ρ α] (m : Raw α (fun _ => Unit)) (l : ρ) : Raw α (fun _ => Unit) :=
+@[inline, inherit_doc Raw.insertMany] def Const.insertManyUnit [BEq α] [Hashable α] {ρ : Type w} [ForIn Id ρ α] (m : Raw α (fun _ => Unit)) (l : ρ) : Raw α (fun _ => Unit) :=
   if h : 0 < m.buckets.size then
     (Raw₀.Const.insertManyUnit ⟨m, h⟩ l).1
   else m -- will never happen for well-formed inputs
 
+/-- Creates a hash map from a list of mappings. -/
 @[inline] def ofList [BEq α] [Hashable α] {ρ : Type w} [ForIn Id ρ ((a : α) × β a)] (l : ρ) : Raw α β :=
   insertMany ∅ l
 
-@[inline] def Const.ofList {β : Type v} [BEq α] [Hashable α] {ρ : Type w} [ForIn Id ρ (α × β)] (l : ρ) : Raw α (fun _ => β) :=
+@[inline, inherit_doc Raw.ofList] def Const.ofList {β : Type v} [BEq α] [Hashable α] {ρ : Type w} [ForIn Id ρ (α × β)] (l : ρ) : Raw α (fun _ => β) :=
   Const.insertMany ∅ l
 
-@[inline] def Const.unitOfList [BEq α] [Hashable α] {ρ : Type w} [ForIn Id ρ α] (l : ρ) : Raw α (fun _ => Unit) :=
+@[inline, inherit_doc Raw.ofList] def Const.unitOfList [BEq α] [Hashable α] {ρ : Type w} [ForIn Id ρ α] (l : ρ) : Raw α (fun _ => Unit) :=
   Const.insertManyUnit ∅ l
 
+/-- Returns the number of buckets in the internal representation of the hash map. This function may
+be useful for things like monitoring system health, but it should be considered an internal
+implementation detail. -/
 def Internal.numBuckets (m : Raw α β) : Nat :=
   m.buckets.size
 
@@ -232,23 +296,34 @@ end Unverified
 section WF
 
 /--
-Well-formedness predicate for hash maps. Users of `DHashMap` will not need to interact with this. Users of `DHashMap.Raw`
-will need to provide proofs of `WF` to lemmas and should use the lemmas `WF.empty`, `WF.emptyc`, `WF.insert`, `WF.containsThenInsert`,
-`WF.remove`, `WF.insertIfNew`, `WF.getThenInsertIfNew?`, `WF.filter`, `WF.Const.getThenInsertIfNew?`, `WF.filterMap` and `WF.map` to
-show that map operations preserve well-formedness.
+Well-formedness predicate for hash maps. Users of `DHashMap` will not need to interact with this.
+Users of `DHashMap.Raw` will need to provide proofs of `WF` to lemmas and should use the lemmas
+`WF.empty`, `WF.emptyc`, `WF.insert`, `WF.containsThenInsert`, `WF.remove`, `WF.insertIfNew`,
+`WF.getThenInsertIfNew?`, `WF.filter`, `WF.Const.getThenInsertIfNew?`, `WF.filterMap` and `WF.map`
+to show that map operations preserve well-formedness. The constructors of this type are internal
+implementation details and should not be accessed by users.
 -/
 inductive WF : {α : Type u} → {β : α → Type v} → [BEq α] → [Hashable α] → Raw α β → Prop where
   -- Implementation note: the reason why we provide the `[EquivBEq α] [LawfulHashable α]` is so that we can write down
   -- `DHashMap.map` and `DHashMap.filterMap` in `AdditionalOperations.lean` without requiring these proofs just to invoke
   -- the operations.
+  /-- Internal implementation detail of the hash map -/
   | wf {α β} [BEq α] [Hashable α] {m : Raw α β} : 0 < m.buckets.size → (∀ [EquivBEq α] [LawfulHashable α], Raw.WFImp m) → WF m
+  /-- Internal implementation detail of the hash map -/
   | empty₀ {α β} [BEq α] [Hashable α] {c} : WF (Raw₀.empty c : Raw₀ α β).1
+  /-- Internal implementation detail of the hash map -/
   | insert₀ {α β} [BEq α] [Hashable α] {m : Raw α β} {h a b} : WF m → WF (Raw₀.insert ⟨m, h⟩ a b).1
+  /-- Internal implementation detail of the hash map -/
   | containsThenInsert₀ {α β} [BEq α] [Hashable α] {m : Raw α β} {h a b} : WF m → WF (Raw₀.containsThenInsert ⟨m, h⟩ a b).2.1
+  /-- Internal implementation detail of the hash map -/
   | remove₀ {α β} [BEq α] [Hashable α] {m : Raw α β} {h a} : WF m → WF (Raw₀.remove ⟨m, h⟩ a).1
+  /-- Internal implementation detail of the hash map -/
   | insertIfNew₀ {α β} [BEq α] [Hashable α] {m : Raw α β} {h a b} : WF m → WF (Raw₀.insertIfNew ⟨m, h⟩ a b).1
+  /-- Internal implementation detail of the hash map -/
   | getThenInsertIfNew?₀ {α β} [BEq α] [Hashable α] [LawfulBEq α] {m : Raw α β} {h a b} : WF m → WF (Raw₀.getThenInsertIfNew? ⟨m, h⟩ a b).2.1
+  /-- Internal implementation detail of the hash map -/
   | filter₀ {α β} [BEq α] [Hashable α] {m : Raw α β} {h f} : WF m → WF (Raw₀.filter f ⟨m, h⟩).1
+  /-- Internal implementation detail of the hash map -/
   | constGetThenInsertIfNew?₀ {α β} [BEq α] [Hashable α] {m : Raw α (fun _ => β)} {h a b} : WF m → WF (Raw₀.Const.getThenInsertIfNew? ⟨m, h⟩ a b).2.1
 
 theorem WF.size_buckets_pos [BEq α] [Hashable α] (m : Raw α β) : WF m → 0 < m.buckets.size
@@ -262,12 +337,10 @@ theorem WF.size_buckets_pos [BEq α] [Hashable α] (m : Raw α β) : WF m → 0 
   | filter₀ _ => (Raw₀.filter _ ⟨_, _⟩).2
   | constGetThenInsertIfNew?₀ _ => (Raw₀.Const.getThenInsertIfNew? ⟨_, _⟩ _ _).2.2
 
-@[simp]
-theorem WF.empty [BEq α] [Hashable α] {c : Nat} : (Raw.empty c : Raw α β).WF :=
+@[simp] theorem WF.empty [BEq α] [Hashable α] {c : Nat} : (Raw.empty c : Raw α β).WF :=
   .empty₀
 
-@[simp]
-theorem WF.emptyc [BEq α] [Hashable α] : (∅ : Raw α β).WF :=
+@[simp] theorem WF.emptyc [BEq α] [Hashable α] : (∅ : Raw α β).WF :=
   .empty
 
 theorem WF.insert [BEq α] [Hashable α] {m : Raw α β} {a : α} {b : β a} (h : m.WF) : (m.insert a b).WF := by
@@ -321,49 +394,35 @@ end Raw
 
 end DHashMap
 
+/-- Dependent hash maps. -/
 def DHashMap (α : Type u) (β : α → Type v) [BEq α] [Hashable α] := { m : DHashMap.Raw α β // m.WF }
 
 namespace DHashMap
 
-/-- Constructs an empty hash map with a number of buckets appropriate for the given size. -/
-@[inline] def empty [BEq α] [Hashable α] (capacity := 8) : DHashMap α β :=
+@[inline, inherit_doc Raw.empty] def empty [BEq α] [Hashable α] (capacity := 8) : DHashMap α β :=
   ⟨Raw.empty capacity, .empty₀⟩
 
 instance [BEq α] [Hashable α] : EmptyCollection (DHashMap α β) where
   emptyCollection := empty
 
-/--
-Inserts the mapping into the map, replacing an existing mapping if there is one.
--/
-@[inline] def insert [BEq α] [Hashable α] (m : DHashMap α β) (a : α) (b : β a) : DHashMap α β :=
+@[inline, inherit_doc Raw.insert] def insert [BEq α] [Hashable α] (m : DHashMap α β) (a : α) (b : β a) : DHashMap α β :=
   ⟨Raw₀.insert ⟨m.1, m.2.size_buckets_pos⟩ a b, .insert₀ m.2⟩
 
-@[inline] def insertIfNew [BEq α] [Hashable α] (m : DHashMap α β) (a : α) (b : β a) : DHashMap α β :=
+@[inline, inherit_doc Raw.insertIfNew] def insertIfNew [BEq α] [Hashable α] (m : DHashMap α β) (a : α) (b : β a) : DHashMap α β :=
   ⟨Raw₀.insertIfNew ⟨m.1, m.2.size_buckets_pos⟩ a b, .insertIfNew₀ m.2⟩
 
-/--
-Inserts the mapping into the map, replacing an existing mapping if there is one.
-Returns `true` if there was a previous mapping that was replaced.
--/
-@[inline] def containsThenInsert [BEq α] [Hashable α] (m : DHashMap α β) (a : α) (b : β a) : Bool × DHashMap α β :=
+@[inline, inherit_doc Raw.containsThenInsert] def containsThenInsert [BEq α] [Hashable α] (m : DHashMap α β) (a : α) (b : β a) : Bool × DHashMap α β :=
   let m' := Raw₀.containsThenInsert ⟨m.1, m.2.size_buckets_pos⟩ a b
   ⟨m'.1, ⟨m'.2.1, .containsThenInsert₀ m.2⟩⟩
 
-@[inline] def getThenInsertIfNew? [BEq α] [Hashable α] [LawfulBEq α] (m : DHashMap α β) (a : α) (b : β a) : Option (β a) × DHashMap α β :=
+@[inline, inherit_doc Raw.getThenInsertIfNew?] def getThenInsertIfNew? [BEq α] [Hashable α] [LawfulBEq α] (m : DHashMap α β) (a : α) (b : β a) : Option (β a) × DHashMap α β :=
   let m' := Raw₀.getThenInsertIfNew? ⟨m.1, m.2.size_buckets_pos⟩ a b
   ⟨m'.1, ⟨m'.2.1, .getThenInsertIfNew?₀ m.2⟩⟩
 
-/--
-Retrieves the value associated with the given key, if it exists. This function requires a `LawfulBEq` instance
-to be able to cast the value to the correct type. If no such instance is available, you can use `getEntry?`,
-`getWithCast?`,
-or switch to a non-dependent `HashMap`.
--/
-@[inline] def get? [BEq α] [LawfulBEq α] [Hashable α] (m : DHashMap α β) (a : α) : Option (β a) :=
+@[inline, inherit_doc Raw.get?] def get? [BEq α] [LawfulBEq α] [Hashable α] (m : DHashMap α β) (a : α) : Option (β a) :=
   Raw₀.get? ⟨m.1, m.2.size_buckets_pos⟩ a
 
-/-- Returns true if the hash map contains a mapping with a key equal to the given key. -/
-@[inline] def contains [BEq α] [Hashable α] (m : DHashMap α β) (a : α) : Bool :=
+@[inline, inherit_doc Raw.contains] def contains [BEq α] [Hashable α] (m : DHashMap α β) (a : α) : Bool :=
   Raw₀.contains ⟨m.1, m.2.size_buckets_pos⟩ a
 
 instance [BEq α] [Hashable α] : Membership α (DHashMap α β) where
@@ -372,69 +431,64 @@ instance [BEq α] [Hashable α] : Membership α (DHashMap α β) where
 instance [BEq α] [Hashable α] {m : DHashMap α β} {a : α} : Decidable (a ∈ m) :=
   show Decidable (m.contains a) from inferInstance
 
-@[inline] def get [BEq α] [Hashable α] [LawfulBEq α] (m : DHashMap α β) (a : α) (h : a ∈ m) : β a :=
+@[inline, inherit_doc Raw.get] def get [BEq α] [Hashable α] [LawfulBEq α] (m : DHashMap α β) (a : α) (h : a ∈ m) : β a :=
   Raw₀.get ⟨m.1, m.2.size_buckets_pos⟩ a h
 
-@[inline] def get! [BEq α] [Hashable α] [LawfulBEq α] (m : DHashMap α β) (a : α) [Inhabited (β a)] : β a :=
+@[inline, inherit_doc Raw.get!] def get! [BEq α] [Hashable α] [LawfulBEq α] (m : DHashMap α β) (a : α) [Inhabited (β a)] : β a :=
   Raw₀.get! ⟨m.1, m.2.size_buckets_pos⟩ a
 
-@[inline] def getD [BEq α] [Hashable α] [LawfulBEq α] (m : DHashMap α β) (a : α) (fallback : β a) : β a :=
+@[inline, inherit_doc Raw.getD] def getD [BEq α] [Hashable α] [LawfulBEq α] (m : DHashMap α β) (a : α) (fallback : β a) : β a :=
   Raw₀.getD ⟨m.1, m.2.size_buckets_pos⟩ a fallback
 
-/--
-Removes the mapping with the given key if it exists.
--/
-@[inline] def remove [BEq α] [Hashable α] (m : DHashMap α β) (a : α) : DHashMap α β :=
+@[inline, inherit_doc Raw.remove] def remove [BEq α] [Hashable α] (m : DHashMap α β) (a : α) : DHashMap α β :=
   ⟨Raw₀.remove ⟨m.1, m.2.size_buckets_pos⟩ a, .remove₀ m.2⟩
 
 section
 
 variable {β : Type v}
 
-/--
-Retrieves the value associated with the given key, if it exists. -/
-@[inline] def Const.get? [BEq α] [Hashable α] (m : DHashMap α (fun _ => β)) (a : α) : Option β :=
+@[inline, inherit_doc Raw.Const.get?] def Const.get? [BEq α] [Hashable α] (m : DHashMap α (fun _ => β)) (a : α) : Option β :=
   Raw₀.Const.get? ⟨m.1, m.2.size_buckets_pos⟩ a
 
-@[inline] def Const.get [BEq α] [Hashable α] (m : DHashMap α (fun _ => β)) (a : α) (h : a ∈ m) : β :=
+@[inline, inherit_doc Raw.Const.get] def Const.get [BEq α] [Hashable α] (m : DHashMap α (fun _ => β)) (a : α) (h : a ∈ m) : β :=
   Raw₀.Const.get ⟨m.1, m.2.size_buckets_pos⟩ a h
 
-@[inline] def Const.getD [BEq α] [Hashable α] (m : DHashMap α (fun _ => β)) (a : α) (fallback : β) : β :=
+@[inline, inherit_doc Raw.Const.getD] def Const.getD [BEq α] [Hashable α] (m : DHashMap α (fun _ => β)) (a : α) (fallback : β) : β :=
   Raw₀.Const.getD ⟨m.1, m.2.size_buckets_pos⟩ a fallback
 
-@[inline] def Const.get! [BEq α] [Hashable α] [Inhabited β] (m : DHashMap α (fun _ => β)) (a : α) : β :=
+@[inline, inherit_doc Raw.Const.get!] def Const.get! [BEq α] [Hashable α] [Inhabited β] (m : DHashMap α (fun _ => β)) (a : α) : β :=
   Raw₀.Const.get! ⟨m.1, m.2.size_buckets_pos⟩ a
 
-@[inline] def Const.getThenInsertIfNew? [BEq α] [Hashable α] (m : DHashMap α (fun _ => β)) (a : α) (b : β) :
+@[inline, inherit_doc Raw.Const.getThenInsertIfNew?] def Const.getThenInsertIfNew? [BEq α] [Hashable α] (m : DHashMap α (fun _ => β)) (a : α) (b : β) :
     Option β × DHashMap α (fun _ => β) :=
   let m' := Raw₀.Const.getThenInsertIfNew? ⟨m.1, m.2.size_buckets_pos⟩ a b
   ⟨m'.1, ⟨m'.2.1, .constGetThenInsertIfNew?₀ m.2⟩⟩
 
 end
 
-@[inline] def size [BEq α] [Hashable α] (m : DHashMap α β) : Nat :=
+@[inline, inherit_doc Raw.size] def size [BEq α] [Hashable α] (m : DHashMap α β) : Nat :=
   m.1.size
 
-@[inline] def isEmpty [BEq α] [Hashable α] (m : DHashMap α β) : Bool :=
+@[inline, inherit_doc Raw.isEmpty] def isEmpty [BEq α] [Hashable α] (m : DHashMap α β) : Bool :=
   m.1.isEmpty
 
 section Unverified
 
 /-! We currently do not provide lemmas for the functions below. -/
 
-@[inline] def filter [BEq α] [Hashable α] (f : (a : α) → β a → Bool) (m : DHashMap α β) : DHashMap α β :=
+@[inline, inherit_doc Raw.filter] def filter [BEq α] [Hashable α] (f : (a : α) → β a → Bool) (m : DHashMap α β) : DHashMap α β :=
   ⟨Raw₀.filter f ⟨m.1, m.2.size_buckets_pos⟩, .filter₀ m.2⟩
 
-@[inline] def foldlM [BEq α] [Hashable α] (f : δ → (a : α) → β a → m δ) (init : δ) (b : DHashMap α β) : m δ :=
+@[inline, inherit_doc Raw.foldlM] def foldlM [BEq α] [Hashable α] (f : δ → (a : α) → β a → m δ) (init : δ) (b : DHashMap α β) : m δ :=
   b.1.foldlM f init
 
-@[inline] def foldl [BEq α] [Hashable α] (f : δ → (a : α) → β a → δ) (init : δ) (b : DHashMap α β) : δ :=
+@[inline, inherit_doc Raw.foldl] def foldl [BEq α] [Hashable α] (f : δ → (a : α) → β a → δ) (init : δ) (b : DHashMap α β) : δ :=
   b.1.foldl f init
 
-@[inline] def forM [BEq α] [Hashable α] (f : (a : α) → β a → m PUnit) (b : DHashMap α β) : m PUnit :=
+@[inline, inherit_doc Raw.forM] def forM [BEq α] [Hashable α] (f : (a : α) → β a → m PUnit) (b : DHashMap α β) : m PUnit :=
   b.1.forM f
 
-@[inline] def forIn [BEq α] [Hashable α] (f : (a : α) → β a → δ → m (ForInStep δ)) (init : δ) (b : DHashMap α β) : m δ :=
+@[inline, inherit_doc Raw.forIn] def forIn [BEq α] [Hashable α] (f : (a : α) → β a → δ → m (ForInStep δ)) (init : δ) (b : DHashMap α β) : m δ :=
   b.1.forIn f init
 
 instance [BEq α] [Hashable α] : ForM m (DHashMap α β) (Σ a, β a) where
@@ -443,46 +497,46 @@ instance [BEq α] [Hashable α] : ForM m (DHashMap α β) (Σ a, β a) where
 instance [BEq α] [Hashable α] : ForIn m (DHashMap α β) (Σ a, β a) where
   forIn m init f := m.forIn (fun a b acc => f ⟨a, b⟩ acc) init
 
-@[inline] def toList [BEq α] [Hashable α] (m : DHashMap α β) : List (Σ a, β a) :=
+@[inline, inherit_doc Raw.toList] def toList [BEq α] [Hashable α] (m : DHashMap α β) : List (Σ a, β a) :=
   m.1.toList
 
-@[inline] def toArray [BEq α] [Hashable α] (m : DHashMap α β) : Array (Σ a, β a) :=
+@[inline, inherit_doc Raw.toArray] def toArray [BEq α] [Hashable α] (m : DHashMap α β) : Array (Σ a, β a) :=
   m.1.toArray
 
-@[inline] def Const.toList {β : Type v} [BEq α] [Hashable α] (m : DHashMap α (fun _ => β)) : List (α × β) :=
+@[inline, inherit_doc Raw.Const.toList] def Const.toList {β : Type v} [BEq α] [Hashable α] (m : DHashMap α (fun _ => β)) : List (α × β) :=
   Raw.Const.toList m.1
 
-@[inline] def Const.toArray {β : Type v} [BEq α] [Hashable α] (m : DHashMap α (fun _ => β)) : Array (α × β) :=
+@[inline, inherit_doc Raw.Const.toArray] def Const.toArray {β : Type v} [BEq α] [Hashable α] (m : DHashMap α (fun _ => β)) : Array (α × β) :=
   Raw.Const.toArray m.1
 
-@[inline] def keys [BEq α] [Hashable α] (m : DHashMap α β) : List α :=
+@[inline, inherit_doc Raw.keys] def keys [BEq α] [Hashable α] (m : DHashMap α β) : List α :=
   m.1.keys
 
-@[inline] def keysArray [BEq α] [Hashable α] (m : DHashMap α β) : Array α :=
+@[inline, inherit_doc Raw.keysArray] def keysArray [BEq α] [Hashable α] (m : DHashMap α β) : Array α :=
   m.1.keysArray
 
-@[inline] def values {β : Type v} [BEq α] [Hashable α] (m : DHashMap α (fun _ => β)) : List β :=
+@[inline, inherit_doc Raw.values] def values {β : Type v} [BEq α] [Hashable α] (m : DHashMap α (fun _ => β)) : List β :=
   m.1.values
 
-@[inline] def insertMany [BEq α] [Hashable α] {ρ : Type w} [ForIn Id ρ ((a : α) × β a)] (m : DHashMap α β) (l : ρ) : DHashMap α β :=
+@[inline, inherit_doc Raw.insertMany] def insertMany [BEq α] [Hashable α] {ρ : Type w} [ForIn Id ρ ((a : α) × β a)] (m : DHashMap α β) (l : ρ) : DHashMap α β :=
   ⟨(Raw₀.insertMany ⟨m.1, m.2.size_buckets_pos⟩ l).1, (Raw₀.insertMany ⟨m.1, m.2.size_buckets_pos⟩ l).2 _ Raw.WF.insert₀ m.2⟩
 
-@[inline] def Const.insertMany {β : Type v} [BEq α] [Hashable α] {ρ : Type w} [ForIn Id ρ (α × β)] (m : DHashMap α (fun _ => β)) (l : ρ) : DHashMap α (fun _ => β) :=
+@[inline, inherit_doc Raw.Const.insertMany] def Const.insertMany {β : Type v} [BEq α] [Hashable α] {ρ : Type w} [ForIn Id ρ (α × β)] (m : DHashMap α (fun _ => β)) (l : ρ) : DHashMap α (fun _ => β) :=
   ⟨(Raw₀.Const.insertMany ⟨m.1, m.2.size_buckets_pos⟩ l).1, (Raw₀.Const.insertMany ⟨m.1, m.2.size_buckets_pos⟩ l).2 _ Raw.WF.insert₀ m.2⟩
 
-@[inline] def Const.insertManyUnit [BEq α] [Hashable α] {ρ : Type w} [ForIn Id ρ α] (m : DHashMap α (fun _ => Unit)) (l : ρ) : DHashMap α (fun _ => Unit) :=
+@[inline, inherit_doc Raw.Const.insertManyUnit] def Const.insertManyUnit [BEq α] [Hashable α] {ρ : Type w} [ForIn Id ρ α] (m : DHashMap α (fun _ => Unit)) (l : ρ) : DHashMap α (fun _ => Unit) :=
   ⟨(Raw₀.Const.insertManyUnit ⟨m.1, m.2.size_buckets_pos⟩ l).1, (Raw₀.Const.insertManyUnit ⟨m.1, m.2.size_buckets_pos⟩ l).2 _ Raw.WF.insert₀ m.2⟩
 
-@[inline] def ofList [BEq α] [Hashable α] {ρ : Type w} [ForIn Id ρ ((a : α) × β a)] (l : ρ) : DHashMap α β :=
+@[inline, inherit_doc Raw.ofList] def ofList [BEq α] [Hashable α] {ρ : Type w} [ForIn Id ρ ((a : α) × β a)] (l : ρ) : DHashMap α β :=
   insertMany ∅ l
 
-@[inline] def Const.ofList {β : Type v} [BEq α] [Hashable α] {ρ : Type w} [ForIn Id ρ (α × β)] (l : ρ) : DHashMap α (fun _ => β) :=
+@[inline, inherit_doc Raw.Const.ofList] def Const.ofList {β : Type v} [BEq α] [Hashable α] {ρ : Type w} [ForIn Id ρ (α × β)] (l : ρ) : DHashMap α (fun _ => β) :=
   Const.insertMany ∅ l
 
-@[inline] def Const.unitOfList [BEq α] [Hashable α] {ρ : Type w} [ForIn Id ρ α] (l : ρ) : DHashMap α (fun _ => Unit) :=
+@[inline, inherit_doc Raw.Const.unitOfList] def Const.unitOfList [BEq α] [Hashable α] {ρ : Type w} [ForIn Id ρ α] (l : ρ) : DHashMap α (fun _ => Unit) :=
   Const.insertManyUnit ∅ l
 
-def Internal.numBuckets [BEq α] [Hashable α] (m : DHashMap α β) :=
+@[inherit_doc Raw.Internal.numBuckets] def Internal.numBuckets [BEq α] [Hashable α] (m : DHashMap α β) : Nat :=
   Raw.Internal.numBuckets m.1
 
 instance [BEq α] [Hashable α] [Repr α] [(a : α) → Repr (β a)] : Repr (DHashMap α β) where
